Switch to reflective bounded word in Ed25519
(cc @andres-erbsen)

src/Specific/GF25519Bounded.v
@@ -7,7 +7,7 @@ Require Import Crypto.ModularArithmetic.ModularBaseSystemProofs.
 Require Import Crypto.ModularArithmetic.ModularBaseSystemOpt.
 Require Import Crypto.Specific.GF25519.
 Require Import Crypto.Specific.GF25519BoundedCommon.
-(*Require Import Crypto.Assembly.GF25519BoundedInstantiation.*)
+Require Import Crypto.Specific.GF25519Reflective.
 Require Import Bedrock.Word Crypto.Util.WordUtil.
 Require Import Coq.Lists.List Crypto.Util.ListUtil.
 Require Import Crypto.Tactics.VerdiTactics.
@@ -45,11 +45,15 @@ Local Ltac define_unop_WireToFE f opW blem :=
   abstract bounded_wire_digits_t opW blem.
 
 Local Opaque Let_In.
-(*Local Arguments interp_radd / _ _.
+Local Opaque Z.add Z.sub Z.mul Z.shiftl Z.shiftr Z.land Z.lor Z.eqb.
+Local Arguments interp_radd / _ _.
 Local Arguments interp_rsub / _ _.
 Local Arguments interp_rmul / _ _.
 Local Arguments interp_ropp / _.
 Local Arguments interp_rfreeze / _.
+Local Arguments interp_rge_modulus / _.
+Local Arguments interp_rpack / _.
+Local Arguments interp_runpack / _.
 Definition addW (f g : fe25519W) : fe25519W := Eval simpl in interp_radd f g.
 Definition subW (f g : fe25519W) : fe25519W := Eval simpl in interp_rsub f g.
 Definition mulW (f g : fe25519W) : fe25519W := Eval simpl in interp_rmul f g.
@@ -57,15 +61,7 @@ Definition oppW (f : fe25519W) : fe25519W := Eval simpl in interp_ropp f.
 Definition freezeW (f : fe25519W) : fe25519W := Eval simpl in interp_rfreeze f.
 Definition ge_modulusW (f : fe25519W) : word64 := Eval simpl in interp_rge_modulus f.
 Definition packW (f : fe25519W) : wire_digitsW := Eval simpl in interp_rpack f.
-Definition unpackW (f : wire_digitsW) : fe25519W := Eval simpl in interp_runpack f.*)
-Definition addW (f g : fe25519W) : fe25519W := Eval cbv beta delta [carry_add] in carry_add f g.
-Definition subW (f g : fe25519W) : fe25519W := Eval cbv beta delta [carry_sub] in carry_sub f g.
-Definition mulW (f g : fe25519W) : fe25519W := Eval cbv beta delta [mul] in mul f g.
-Definition oppW (f : fe25519W) : fe25519W := Eval cbv beta delta [carry_opp] in carry_opp f.
-Definition freezeW (f : fe25519W) : fe25519W := Eval cbv beta delta [freeze] in freeze f.
-Definition ge_modulusW (f : fe25519W) : word64 := Eval cbv beta delta [ge_modulus] in ge_modulus f.
-Definition packW (f : fe25519W) : wire_digitsW := Eval cbv beta delta [pack] in pack f.
-Definition unpackW (f : wire_digitsW) : fe25519W := Eval cbv beta delta [unpack] in unpack f.
+Definition unpackW (f : wire_digitsW) : fe25519W := Eval simpl in interp_runpack f.
 
 Local Transparent Let_In.
 Definition powW (f : fe25519W) chain := fold_chain_opt (proj1_fe25519W one) mulW chain [f].
@@ -78,21 +74,21 @@ Local Ltac port_correct_and_bounded pre_rewrite opW interp_rop rop_cb :=
   intros; apply rop_cb; assumption.
 
 Lemma addW_correct_and_bounded : ibinop_correct_and_bounded addW carry_add.
-Proof. (*port_correct_and_bounded interp_radd_correct addW interp_radd radd_correct_and_bounded. Qed.*) Admitted.
+Proof. port_correct_and_bounded interp_radd_correct addW interp_radd radd_correct_and_bounded. Qed.
 Lemma subW_correct_and_bounded : ibinop_correct_and_bounded subW carry_sub.
-Proof. (*port_correct_and_bounded interp_rsub_correct subW interp_rsub rsub_correct_and_bounded. Qed.*) Admitted.
+Proof. port_correct_and_bounded interp_rsub_correct subW interp_rsub rsub_correct_and_bounded. Qed.
 Lemma mulW_correct_and_bounded : ibinop_correct_and_bounded mulW mul.
-Proof. (*port_correct_and_bounded interp_rmul_correct mulW interp_rmul rmul_correct_and_bounded. Qed.*) Admitted.
+Proof. port_correct_and_bounded interp_rmul_correct mulW interp_rmul rmul_correct_and_bounded. Qed.
 Lemma oppW_correct_and_bounded : iunop_correct_and_bounded oppW carry_opp.
-Proof. (*port_correct_and_bounded interp_ropp_correct oppW interp_ropp ropp_correct_and_bounded. Qed.*) Admitted.
+Proof. port_correct_and_bounded interp_ropp_correct oppW interp_ropp ropp_correct_and_bounded. Qed.
 Lemma freezeW_correct_and_bounded : iunop_correct_and_bounded freezeW freeze.
-Proof. (*port_correct_and_bounded interp_rfreeze_correct freezeW interp_rfreeze rfreeze_correct_and_bounded. Qed.*) Admitted.
+Proof. port_correct_and_bounded interp_rfreeze_correct freezeW interp_rfreeze rfreeze_correct_and_bounded. Qed.
 Lemma ge_modulusW_correct : iunop_FEToZ_correct ge_modulusW ge_modulus.
-Proof. (*port_correct_and_bounded interp_rge_modulus_correct ge_modulusW interp_rge_modulus rge_modulus_correct_and_bounded. Qed.*) Admitted.
+Proof. port_correct_and_bounded interp_rge_modulus_correct ge_modulusW interp_rge_modulus rge_modulus_correct_and_bounded. Qed.
 Lemma packW_correct_and_bounded : iunop_FEToWire_correct_and_bounded packW pack.
-Proof. (*port_correct_and_bounded interp_rpack_correct packW interp_rpack rpack_correct_and_bounded. Qed.*) Admitted.
+Proof. port_correct_and_bounded interp_rpack_correct packW interp_rpack rpack_correct_and_bounded. Qed.
 Lemma unpackW_correct_and_bounded : iunop_WireToFE_correct_and_bounded unpackW unpack.
-Proof. (*port_correct_and_bounded interp_runpack_correct unpackW interp_runpack runpack_correct_and_bounded. Qed.*) Admitted.
+Proof. port_correct_and_bounded interp_runpack_correct unpackW interp_runpack runpack_correct_and_bounded. Qed.
 
 Lemma powW_correct_and_bounded chain : iunop_correct_and_bounded (fun x => powW x chain) (fun x => pow x chain).
 Proof.
@@ -100,8 +96,7 @@ Proof.
   intro x; intros; apply (fold_chain_opt_gen fe25519WToZ is_bounded [x]).
   { reflexivity. }
   { reflexivity. }
-  { intros; progress rewrite <- ?mul_correct,
-            <- ?(fun X Y => proj1 (mulW_correct_and_bounded _ _ X Y)) by assumption.
+  { intros; progress rewrite <- (fun X Y => proj1 (mulW_correct_and_bounded _ _ X Y)) by assumption.
     apply mulW_correct_and_bounded; assumption. }
   { intros; rewrite (fun X Y => proj1 (mulW_correct_and_bounded _ _ X Y)) by assumption; reflexivity. }
   { intros [|?]; autorewrite with simpl_nth_default;
@@ -204,7 +199,8 @@ Proof.
       apply Proper_Let_In_nd_changebody_eq; intros.
       set_evars.
       change sqrt_m1 with (fe25519WToZ sqrt_m1W).
-      rewrite <- !(fun X Y => proj1 (mulW_correct_and_bounded _ _ X Y)), <- eqbW_correct, (pull_bool_if fe25519WToZ)
+      rewrite <- (fun X Y => proj1 (mulW_correct_and_bounded a a X Y)),
+      <- (fun X Y => proj1 (mulW_correct_and_bounded sqrt_m1W a X Y)), <- eqbW_correct, (pull_bool_if fe25519WToZ)
         by repeat match goal with
                   | _ => progress subst
                   | [ |- is_bounded (fe25519WToZ ?op) = true ]
