src/Specific/GF25519Reflective/Common.v
@@ -1,5 +1,5 @@
 Require Export Crypto.Specific.GF25519.
-Require Import Crypto.Specific.GF25519BoundedCommonWord.
+Require Import Crypto.Specific.GF25519BoundedCommon.
 Require Import Crypto.Reflection.Reify.
 Require Import Crypto.Reflection.Syntax.
 Require Import Crypto.Reflection.Z.Interpretations.
@@ -37,15 +37,15 @@ Definition ExprUnOpFEToZ : Type := Expr ExprUnOpFEToZT.
 Definition ExprUnOpWireToFE : Type := Expr ExprUnOpWireToFET.
 Definition ExprUnOpFEToWire : Type := Expr ExprUnOpFEToWireT.
 
-Definition interp_bexpr : ExprBinOp -> Specific.GF25519BoundedCommonWord.fe25519W -> Specific.GF25519BoundedCommonWord.fe25519W -> Specific.GF25519BoundedCommonWord.fe25519W
+Definition interp_bexpr : ExprBinOp -> Specific.GF25519BoundedCommon.fe25519W -> Specific.GF25519BoundedCommon.fe25519W -> Specific.GF25519BoundedCommon.fe25519W
   := fun e => curry_binop_fe25519W (Interp (@Word64.interp_op) e).
-Definition interp_uexpr : ExprUnOp -> Specific.GF25519BoundedCommonWord.fe25519W -> Specific.GF25519BoundedCommonWord.fe25519W
+Definition interp_uexpr : ExprUnOp -> Specific.GF25519BoundedCommon.fe25519W -> Specific.GF25519BoundedCommon.fe25519W
   := fun e => curry_unop_fe25519W (Interp (@Word64.interp_op) e).
-Definition interp_uexpr_FEToZ : ExprUnOpFEToZ -> Specific.GF25519BoundedCommonWord.fe25519W -> Specific.GF25519BoundedCommonWord.word64
+Definition interp_uexpr_FEToZ : ExprUnOpFEToZ -> Specific.GF25519BoundedCommon.fe25519W -> Specific.GF25519BoundedCommon.word64
   := fun e => curry_unop_fe25519W (Interp (@Word64.interp_op) e).
-Definition interp_uexpr_FEToWire : ExprUnOpFEToWire -> Specific.GF25519BoundedCommonWord.fe25519W -> Specific.GF25519BoundedCommonWord.wire_digitsW
+Definition interp_uexpr_FEToWire : ExprUnOpFEToWire -> Specific.GF25519BoundedCommon.fe25519W -> Specific.GF25519BoundedCommon.wire_digitsW
   := fun e => curry_unop_fe25519W (Interp (@Word64.interp_op) e).
-Definition interp_uexpr_WireToFE : ExprUnOpWireToFE -> Specific.GF25519BoundedCommonWord.wire_digitsW -> Specific.GF25519BoundedCommonWord.fe25519W
+Definition interp_uexpr_WireToFE : ExprUnOpWireToFE -> Specific.GF25519BoundedCommon.wire_digitsW -> Specific.GF25519BoundedCommon.fe25519W
   := fun e => curry_unop_wire_digitsW (Interp (@Word64.interp_op) e).
 
 Notation binop_correct_and_bounded rop op
